Trace equivalence completed

theories/TraceEquiv.v
@@ -1322,23 +1322,41 @@ actually they should be doubled*)
   (* FIXME: fix statement by adding the fact that continuations != l do not change (and therefore we know
      their projection)
   *)
+
+  Definition R_all_except (l' : lbl) (R : ig_ty -> rl_ty -> Prop)
+             (C : lbl /-> mty * ig_ty) (lC : lbl /-> mty * rl_ty) :=
+    forall l Ty G L,
+      l' != l -> C l = Some (Ty, G) -> lC l = Some (Ty, L) -> R G L.
+
+  Definition updC (l : lbl) (Ty : mty) C E p l' :=
+    if l == l' then
+      Some (Ty, look E p)
+    else
+      C l'.
+
+  Lemma dom_updC l Ty C E p L' :
+    C l = Some (Ty, L') ->
+    same_dom C (updC l Ty C E p).
+  Proof.
+    move=>Cl l1 Ty1;split=>[][G]; rewrite/updC; case: ifP=>EQ.
+    + by move: EQ=>/eqP<-; rewrite Cl=>[][<- _]; exists (look E p).
+    + by move=>->; exists G.
+    + by move: EQ=>/eqP<-; move=>[<-]; exists L'.
+    + by move=>->; exists G.
+  Qed.
+
   Lemma Proj_recv_undo l F T C lCT Ty P G Q' :
     F != T ->
     C l = Some (Ty, G) ->
     look P.lbl T = rl_msg l_recv F lCT ->
     same_dom C lCT ->
+    R_all_except l (IProj T) C lCT ->
     deq P.2 (F, T) = Some (l, Ty, Q') ->
-    (forall p, exists lC,
-          same_dom C lC /\
-          (forall l' Ty' G' L',
-              l != l' ->
-              C l' = Some (Ty', G') ->
-              lC l' = Some (Ty', L') ->
-              IProj p G' L'))  ->
+    (forall p, exists lC, same_dom C lC /\ R_all_except l (IProj p) C lC)  ->
     Projection G (run_step (mk_act l_recv T F l Ty) P) ->
     Projection (ig_msg (Some l) F T C) P.
   Proof.
-    move=> FT Cl ET DOM PFT PRJ0 PRJ1; split.
+    move=> FT Cl ET DOM ALLT PFT PRJ0 PRJ1; split.
     - move=>p; case: (boolP (p == T))=>[/eqP->|pT].
       + move: FT; rewrite eq_sym ET=>TF.
         apply (iprj_recv (Some l) TF)=>// l0 Ty0 G0 L0 Cl0 lCT0.
@@ -1346,23 +1364,23 @@ actually they should be doubled*)
         move: (dom DOM Cl)=>[LT] lCTl; rewrite lCTl !eq_refl /= look_same=>PRJ.
         case: (boolP (l == l0)) => [/eqP|]ll0.
         * by move: ll0 Cl0 lCT0=><-; rewrite Cl lCTl =>[][<-]<-[<-] //.
-        * move: (PRJ0 T)=>[lC'] [DOM'] H; apply/(H _ _ _ _ ll0).
-
-          admit.
-
-      + move: (buildC C P.1) => Cp.
-        admit.
-        admit.
+        * by apply/(ALLT _ _ _ _ ll0 Cl0).
+      + move: (PRJ0 p)=>[lCp] [DOMp] ALLp.
+        move: (dom DOMp Cl) => [Lp] lCpl.
+        move: (dom_updC P.1 p lCpl)=>DOMp'.
+        move: (same_dom_trans DOMp DOMp')=>{}DOMp'.
+        apply: (iprj_send2 pT FT DOMp'); last by rewrite /updC eq_refl.
+        move=> l0 Ty0 G0 G'; rewrite /updC.
+        case: (boolP (l == l0))=>[/eqP<-|NEQ].
+        * move=> Cl0 [EQ_Ty] <-; move: Cl0; rewrite Cl=>[][_ <-].
+          move: (PRJ1.1 p); rewrite /run_step/= ET.
+          move: (dom DOM Cl)=>[LT] lCTl; rewrite lCTl !eq_refl /= look_comm //.
+          by rewrite eq_sym.
+        * by apply/(ALLp l0 Ty0 G0 G' NEQ).
     - move: PFT=>/eqP-PFT; apply: (qprj_some Cl PFT).
       move: PFT=>/eqP-PFT; move: (dom DOM Cl)=>[L] lCtl.
       by move: PRJ1.2; rewrite /run_step/= ET lCtl !eq_refl/= PFT.
-  Admitted.
-
-  Definition updC (l : lbl) (Ty : mty) C E p l' :=
-    if l == l' then
-      Some (Ty, look E p)
-    else
-      C l'.
+  Qed.
 
   (* Not quite right yet *)
   Lemma  proj_same l C0 C1 F T E :
@@ -1417,16 +1435,18 @@ actually they should be doubled*)
       by apply: Ih; [apply: C0l | apply: C1l |].
     - move: Ih=>[SAME_C] [Tyl] [G0] [G1] [C0l] [C1l] [STEP_G0_G1] Ih.
       move: (Projection_runnable C0l PRJ) => RUN.
-      move: (IProj_recv_inv (PRJ.1 T))=>[FT] [lCT] [ET] [DOMT] _.
+      move: (IProj_recv_inv (PRJ.1 T))=>[FT] [lCT] [ET] [DOMT] PRJT.
       move: ET; rewrite -(look_act _ aT)=>{}ET.
       move _: DOM=> DOM1; move: DOM1=>/same_dom_sym-DOM1.
       move: (same_dom_trans DOM1 DOMT)=>{}DOMT.
       move: PRJ.2=>/qProject_Some_inv-[Ty] [G2] [Q'] [].
       rewrite C0l=>[][<-<-] [/eqP/(deq_act aT)-DEQ] _ {Ty G2}.
       move: (proj_same DOM SAME_C PRJ.1)=>PRJ_C1.
-      move: PRJ=>/Proj_Some_next/(_ _ _ C0l)/Ih.
+      move: (Proj_Some_next PRJ)=>/(_ _ _ C0l)/Ih.
       rewrite run_stepC ?RUN ?orbT // => {}Ih.
-      by apply (Proj_recv_undo FT C1l ET DOMT DEQ PRJ_C1).
+      apply: (Proj_recv_undo FT C1l ET DOMT _ DEQ PRJ_C1)=>//.
+      move=>l0 Ty0 G2 L ll0 /(SAME_C _ _ ll0)-Cl0 lCT0.
+      by apply/(PRJT _ _ _ _ Cl0).
     - by apply/Ih/Projection_unr.
   Qed.
 
